examples/dynamic_isolation/TrivialCore.v
@@ -9,10 +9,8 @@ Module EmptyCore (External: External_sig) (Params: EnclaveParameters) (CoreParam
                  <: Core_sig External Params CoreParams.
   Import Common.
 
-  Inductive internal_reg_t' : Type :=
+  Inductive internal_reg_t : Type :=
   | Foo | Bar.
-
-  Definition internal_reg_t := internal_reg_t'.
 
   Definition R_internal (idx: internal_reg_t) : type :=
     match idx with
@@ -24,65 +22,22 @@ Module EmptyCore (External: External_sig) (Params: EnclaveParameters) (CoreParam
     | _ => Bits.zero
     end.
 
-  Inductive external_reg_t :=
-  | core_id
-  | toIMem (state: MemReq.reg_t)
-  | toDMem (state: MemReq.reg_t)
-  | fromIMem (state: MemResp.reg_t)
-  | fromDMem (state: MemResp.reg_t)
-  | toSMEnc (state: EnclaveReq.reg_t)
-  | rf (state: Rf.reg_t)
-  | pc
-  | purge
-  .
+  Instance FiniteType_internal_reg_t : FiniteType internal_reg_t := _.
 
-  Definition R_external (idx: external_reg_t) : type :=
-    match idx with
-    | core_id => core_id_t
-    | toIMem r => MemReq.R r
-    | toDMem r => MemReq.R r
-    | fromIMem  r => MemResp.R r
-    | fromDMem  r => MemResp.R r
-    | toSMEnc r => EnclaveReq.R r
-    | rf r => Rf.R r
-    | pc => bits_t 32
-    | purge => enum_t purge_state
-    end.
+  Definition internal_params : internal_module_sig :=
+    {| _internal_reg_t := internal_reg_t;
+       _R_internal := R_internal;
+       _r_internal := r_internal;
+       _FiniteType_internal_reg_t := FiniteType_internal_reg_t
+    |}.
 
-  Definition r_external (idx: external_reg_t) : R_external idx :=
-    match idx with
-    | core_id => CoreParams.core_id
-    | toIMem s => MemReq.r s
-    | fromIMem s => MemResp.r s
-    | toDMem s => MemReq.r s
-    | fromDMem s => MemResp.r s
-    | toSMEnc s => EnclaveReq.r s
-    | rf r => Rf.r r
-    | pc => CoreParams.initial_pc
-    | purge => value_of_bits (Bits.zero)
-    end.
-
-  Inductive reg_t :=
-  | external (r: external_reg_t)
-  | internal (r: internal_reg_t)
-  .
-
-  Definition R (idx: reg_t) : type :=
-   match idx with
-   | external r => R_external r
-   | internal r => R_internal r
-   end.
-
-  Definition r idx : R idx :=
-    match idx with
-    | external s => r_external s
-    | internal s => r_internal s
-    end.
-
-  Definition ext_fn_t := _ext_fn_t External.ext.
-  Definition Sigma := _Sigma External.ext.
-  Definition rule := rule R Sigma.
-  Definition sigma := _sigma External.ext.
+  Definition reg_t := @Core_Common.reg_t internal_params.
+  Definition r := @Core_Common.r CoreParams.core_id CoreParams.initial_pc internal_params.
+  Definition R := @Core_Common.R internal_params.
+  Definition rule := @Core_Common.rule internal_params External.ext.
+  Definition sigma := @Core_Common.sigma External.ext.
+  Definition Sigma := @Core_Common.Sigma External.ext.
+  Definition ext_fn_t := @Core_Common.ext_fn_t External.ext.
 
   Inductive rule_name_t' : Type := DoNothing | StillDoNothing.
   Definition rule_name_t := rule_name_t'.
@@ -98,367 +53,18 @@ Module EmptyCore (External: External_sig) (Params: EnclaveParameters) (CoreParam
 
   Definition schedule : Syntax.scheduler pos_t rule_name_t := done.
 
-  Instance FiniteType_internal_reg_t : FiniteType internal_reg_t := _.
-  Instance FiniteType_ext_reg_t : FiniteType external_reg_t := _.
-  Instance FiniteType_reg_t : FiniteType reg_t := _.
-  Instance EqDec_reg_t : EqDec reg_t := _.
-
-  Section CycleSemantics.
-    Definition state := env_t ContextEnv (fun idx : reg_t => R idx).
-    Definition empty_log : Log R ContextEnv := log_empty.
-    Definition initial_state := ContextEnv.(create) r.
-
-    Definition update_function : state -> Log R ContextEnv -> Log R ContextEnv :=
-      fun st log => interp_scheduler_delta st sigma rules log schedule.
-
-    Definition log_t := Log R ContextEnv.
-    Definition input_t := Log R_external ContextEnv.
-    Definition output_t := Log R ContextEnv.
-    Definition feedback_t := Log R_external ContextEnv.
-
-    Record step_io :=
-      { step_input : input_t;
-        step_feedback: feedback_t
-      }.
-
-    Definition lift_ext_log (log: Log R_external ContextEnv) : Log R ContextEnv :=
-      ContextEnv.(create) (fun reg => match reg return (RLog (R reg)) with
-                                   | external s => ContextEnv.(getenv) log s
-                                   | _ => []
-                                   end).
-
-    Definition do_step_input__koika (st: state) (ext_input: input_t) : output_t * log_t :=
-       let input := lift_ext_log ext_input in
-       let output := update_function st input in
-       (output, log_app output input).
-
-    Definition do_step__koika (st: state) (step: step_io)
-                            : state * Log R ContextEnv :=
-      let '(output, acc) := do_step_input__koika st step.(step_input) in
-      let final := log_app (lift_ext_log step.(step_feedback)) acc in
-      (commit_update st final, output).
-
-    Definition do_steps__koika (steps: list step_io)
-                             : state * list (Log R ContextEnv) :=
-      fold_left (fun '(st, evs) step =>
-                   let '(st', ev) := do_step__koika st step in
-                   (st', evs ++ [ev]))
-                steps (initial_state, []).
-
-  End CycleSemantics.
-
-  Section Interface.
-    Definition proj_log__ext (log: Log R ContextEnv) : Log R_external ContextEnv :=
-      ContextEnv.(create) (fun reg => ContextEnv.(getenv) log (external reg)).
-
-      Definition tau := Log R_external ContextEnv.
-      Definition trace := list tau.
-  End Interface.
-
-  Section Spec.
-
-    Definition is_external_log (log: Log R ContextEnv) : Prop :=
-      forall reg, match reg with
-             | external r => True
-             | internal r => ContextEnv.(getenv) log reg = []
-             end.
-
-    (* TODO: to simplify for now, we say that the Core executes first *)
-    Definition valid_input_log__common (input_log: Log R_external ContextEnv) : Prop :=
-      input_log = log_empty.
-
-    Definition valid_output_log__common (output_log: Log R ContextEnv) : Prop :=
-      True.
-
-    Definition valid_feedback_log__common (log: Log R_external ContextEnv) : Prop :=
-      (* Writeback to external registers only *)
-      latest_write log core_id = None /\
-      (* TODO: Register file is really internal... we just wanted to be able to talk about it *)
-      (forall s, latest_write log (rf s) = None).
-    (*
-      (latest_write log (external (toIMem MemReq.valid0)) = None \/
-      latest_write log (external (toIMem MemReq.valid0)) = Some Ob~0).
-      *)
-
-    (* - While running, SM only gets to write purging (which doesn't change anything)
-     * - Only Core writes purged, transitioning from running -> waiting
-     * - Here, Core promises to not change external state
-     * - Supposing that SM writes restart only when external state is cleared (apart from certain regs),
-     * - Then simulation of resetting holds.
-     *)
-    Inductive phase_state :=
-    | SpecSt_Running
-    | SpecSt_Waiting (rf: env_t ContextEnv Rf.R)
-    .
-
-    Definition spec_state_t : Type := state * phase_state.
-
-    Definition initial_spec_state : spec_state_t := (initial_state, SpecSt_Running).
-
-    Definition only_write_ext_purge (log: Log R_external ContextEnv) (v: bits_t 2) : Prop :=
-      latest_write log purge = Some v \/ latest_write log purge = None.
-
-    Definition only_write_purge (log: Log R ContextEnv) (v: bits_t 2) : Prop :=
-      latest_write log (external purge) = Some v \/ latest_write log (external purge) = None.
-
-    Definition extract_rf (st: state) : env_t ContextEnv Rf.R :=
-      ContextEnv.(create) (fun reg => ContextEnv.(getenv) st (external (rf reg))).
-
-    Definition initialise_with_rf (initial_rf: env_t ContextEnv Rf.R) (initial_pc: bits_t 32) : state :=
-      ContextEnv.(create) (fun reg => match reg return R reg with
-                                   | external (rf s) => ContextEnv.(getenv) initial_rf s
-                                   | external pc => initial_pc
-                                   | s => r s
-                                   end).
-
-    Definition do_step_trans_input__spec (spec_st: spec_state_t) (ext_input: input_t) : output_t * log_t :=
-      do_step_input__koika (fst spec_st) ext_input.
-
-    (* TODO: should really be inductive probably or option type? But too much effort to specify everything. *)
-    Definition do_step_trans__spec (spec_st: spec_state_t) (step: step_io)
-                           : spec_state_t * Log R ContextEnv :=
-      let '(st, phase) := spec_st in
-      let '(st', output) := do_step__koika st step in
-      let final_st :=
-        match phase with
-        | SpecSt_Running =>
-            let continue := (st', SpecSt_Running) in
-            match latest_write output (external purge) with
-            | Some v => if bits_eqb v ENUM_purge_purged
-                       then (st', SpecSt_Waiting (extract_rf st'))
-                       else continue
-            | None => continue
-            end
-        | SpecSt_Waiting _rf =>
-           let continue := (st', SpecSt_Waiting _rf) in
-           match latest_write step.(step_feedback) purge,
-                 latest_write step.(step_feedback) pc with
-           | Some v, Some _pc =>
-               if bits_eqb v ENUM_purge_restart then
-                 ((initialise_with_rf _rf _pc), SpecSt_Running)
-               else (* don't care *) continue
-           | _, _ => continue
-           end
-        end in
-      (final_st, output).
-
-    (* Behaves nicely with enq/deqs *)
-    Definition valid_interface_log (st: state) (init_log: Log R_external ContextEnv)
-                                   (log: Log R_external ContextEnv) : Prop. Admitted.
-
-    Definition no_writes (log: Log R_external ContextEnv) : Prop :=
-      forall r, latest_write log r = None.
-
-    Definition valid_step_output__spec (spec_st: spec_state_t) (step: step_io) : Prop :=
-      let '(st, phase) := spec_st in
-      let '(st', log) := do_step_trans__spec spec_st step in
-      valid_output_log__common log /\
-      valid_interface_log st log_empty (proj_log__ext log) /\
-        (match phase with
-        | SpecSt_Running => True
-        | SpecSt_Waiting _ =>
-            no_writes (proj_log__ext log)
-        end).
-
-    Definition reset_external_state (st: state) : Prop :=
-      forall reg, match reg with
-             | rf _ => True
-             | pc => True
-             | purge => True
-             | s => ContextEnv.(getenv) st (external s) = r_external s
-             end.
-
-    Definition valid_step_feedback__spec (spec_st: spec_state_t) (step: step_io) : Prop :=
-      let '(st, phase) := spec_st in
-      let '(st', output) := do_step_trans__spec spec_st step in
-      let feedback := step.(step_feedback) in
-
-      valid_feedback_log__common step.(step_feedback) /\
-      valid_interface_log st (log_app (proj_log__ext output) step.(step_input)) feedback /\
-      match phase with
-      | SpecSt_Running =>
-          only_write_ext_purge feedback ENUM_purge_purging
-      | SpecSt_Waiting _  =>
-          only_write_ext_purge feedback ENUM_purge_restart /\
-          (latest_write feedback purge = Some ENUM_purge_restart ->
-           latest_write feedback pc <> None /\
-           reset_external_state (fst st') (* TODO: whose responsibility to clear FIFOs? *)
-          )
-      end.
-
-    Definition do_step__spec (spec_st: spec_state_t) (step: step_io)
-                           : spec_state_t * Log R ContextEnv * props_t :=
-      let '(st', log) := do_step_trans__spec spec_st step in
-      let props' := {| P_input := valid_input_log__common step.(step_input);
-                       P_output := valid_step_output__spec spec_st step;
-                       P_feedback := valid_step_feedback__spec spec_st step
-                    |} in
-      (st', log, props').
-
-    Definition do_steps__spec (steps: list step_io)
-                            : spec_state_t * list (Log R ContextEnv) * list props_t :=
-      fold_left (fun '(st, evs, props) step =>
-                   let '(st', ev, prop) := do_step__spec st step in
-                   (st', evs ++ [ev], props ++ [prop]))
-                steps (initial_spec_state, [], []).
-
-  End Spec.
-
-  Section Correctness.
-
-    (* TODO: clean *)
-
-    Definition ext_log_equivalent (log0 log1: Log R_external ContextEnv) : Prop.
-    Admitted.
-
-    Definition log_equivalent (koika_log: Log R ContextEnv) (spec_log: Log R ContextEnv) : Prop :=
-      forall (reg: external_reg_t),
-        latest_write koika_log (external reg) = latest_write spec_log (external reg) /\
-        (forall port, may_read koika_log port (external reg) = may_read spec_log port (external reg)) /\
-        (forall port, may_write koika_log log_empty port (external reg) =
-                 may_write spec_log log_empty port (external reg)).
-
-    Definition trace_equivalent (koika_tr: list (Log R ContextEnv))
-                                (spec_tr: list (Log R ContextEnv)) : Prop :=
-      Forall2 log_equivalent koika_tr spec_tr.
-
-    Axiom output_correctness:
-      forall (steps: list step_io)
-        (spec_st: spec_state_t) (spec_tr: list (Log R ContextEnv)) (props: list props_t)
-        (koika_st: state) (koika_tr: list (Log R ContextEnv))
-        (input: input_t) (output0 output1: output_t),
-        valid_inputs props ->
-        valid_feedback props ->
-        do_steps__spec steps = (spec_st, spec_tr, props) ->
-        do_steps__koika steps = (koika_st, koika_tr) ->
-        fst (do_step_input__koika koika_st input) = output0 ->
-        fst (do_step_trans_input__spec spec_st input) = output1 ->
-        ext_log_equivalent (proj_log__ext output0) (proj_log__ext output1).
-
-    Axiom correctness :
-      forall (steps: list step_io)
-        (spec_st: spec_state_t) (spec_tr: list (Log R ContextEnv)) (props: list props_t)
-        (koika_st: state) (koika_tr: list (Log R ContextEnv)),
-      valid_inputs props ->
-      valid_feedback props ->
-      do_steps__spec steps = (spec_st, spec_tr, props) ->
-      do_steps__koika steps = (koika_st, koika_tr) ->
-      trace_equivalent koika_tr spec_tr.
-
-  End Correctness.
-
-  Section Compliance.
-    Axiom compliance:
-      forall (steps: list step_io)
-        (spec_st: spec_state_t) (spec_tr: list (Log R ContextEnv)) (props: list props_t)
-        (koika_st: state) (koika_tr: list (Log R ContextEnv)),
-      valid_inputs props ->
-      valid_feedback props ->
-      do_steps__spec steps = (spec_st, spec_tr, props) ->
-      do_steps__koika steps = (koika_st, koika_tr) ->
-      valid_output props.
-
-  End Compliance.
-
-  (* TODO: code duplication *)
-
-  (*
-  Section Constraints.
-    Definition state := env_t ContextEnv (fun idx : reg_t => R idx).
-    Definition empty_log : Log R ContextEnv := log_empty.
-
-    Definition update_function : state -> Log R ContextEnv -> Log R ContextEnv. Admitted.
-
-    Definition update_no_writes_to_reg (st: state) (log: Log R ContextEnv) (reg: reg_t) : Prop :=
-      latest_write (update_function st log) reg = latest_write log reg.
-
-    Definition internal_reg_reset (st: state) (reg: internal_reg_t) : Prop :=
-      ContextEnv.(getenv) st (internal reg) = r (internal reg).
-
-
-    Definition reg_reset (st: state) (reg: reg_t) : Prop :=
-      match reg with
-      | external pc => True (* don't care *)
-      | external purge => True (* don't care *)
-      | external internal s => internal_reg_reset st s
-      | _ => ContextEnv.(getenv) st reg = r reg
-      end.
-
-    Definition valid_reset_state (st: state) : Prop :=
-      forall reg, reg_reset st reg.
-
-    Inductive purge_state_machine (st: state) (log: Log R ContextEnv): Prop :=
-    | PurgeRestart :
-        forall (purge_state_eq: ContextEnv.(getenv) st purge = ENUM_purge_restart)
-          (no_writes_or_write_ready:
-             update_no_writes_to_reg st log purge \/
-             latest_write (update_function st log) purge = Some ENUM_purge_ready),
-          purge_state_machine st log
-    | PurgeReady :
-        forall (purge_state_eq: ContextEnv.(getenv) st purge = ENUM_purge_ready)
-          (no_writes: update_no_writes_to_reg st log purge),
-          purge_state_machine st log
-    | PurgePurging :
-        forall (purge_state_eq: ContextEnv.(getenv) st purge = ENUM_purge_purging)
-          (no_writes_or_write_purged:
-             update_no_writes_to_reg st log purge \/
-             latest_write (update_function st log) purge = Some ENUM_purge_purged
-          ),
-          purge_state_machine st log
-    | PurgePurged :
-        forall (purge_state_eq: ContextEnv.(getenv) st purge = ENUM_purge_purged)
-          (no_writes_to_any_reg: forall reg, update_no_writes_to_reg st log reg),
-          purge_state_machine st log
-    .
-
-    Definition valid_core_id (st: state) : Prop :=
-      ContextEnv.(getenv) st core_id = r core_id.
-
-    Definition valid_state_by_purge (st: state) : Prop :=
-      ContextEnv.(getenv) st purge = ENUM_purge_restart \/
-      ContextEnv.(getenv) st purge = ENUM_purge_purged ->
-      valid_reset_state st.
-
-    Definition valid_internal_state : state -> Prop. Admitted.
-
-    Definition valid_input_log (log: Log R ContextEnv) :=
-      log = empty_log.
-
-    Definition valid_state (st: state) : Prop :=
-      valid_core_id st /\
-      valid_state_by_purge st /\
-      valid_internal_state st.
-
-
-    Axiom valid_state_preserved:
-      forall (st: state) (log: Log R ContextEnv),
-      valid_state st ->
-      valid_input_log log ->
-      valid_state (commit_update st (update_function st log)).
-
-    (* TODO: and valid_state_preserved after external world effects on FIFO? *)
-
-    (* Core_id is unchanged *)
-    Axiom core_id_unchanged :
-      forall (st: state) (log: Log R ContextEnv),
-      latest_write (update_function st log) core_id = latest_write log core_id.
-
-    Axiom valid_purge_state_machine :
-      forall (st: state) (log: Log R ContextEnv),
-        purge_state_machine st log.
-
-    (* If we are in a valid state and write Purging->Purged, then we promise to be in a reset state.
-     * This is a stronger statement that we ultimately need, but is easier to phrase/work with.
-     * I think with modules (/being written in a more modular way without register sharing) this will be easier.
-     *)
-    Axiom write_purged_impl_in_reset_state :
-      forall (st: state) (log: Log R ContextEnv),
-      latest_write (update_function st log) purge = Some ENUM_purge_purged ->
-      latest_write log purge <> Some ENUM_purge_purged ->
-      valid_reset_state (commit_update st (update_function st log)).
-
-
-  End Constraints.
-  *)
+  Instance FiniteType_reg_t : FiniteType reg_t := @Core_Common.FiniteType_reg_t internal_params.
+
+  (* TODO: clean up instantiation *)
+  Parameter output_correctness :
+    @Core_Common.P_output_correctness CoreParams.core_id CoreParams.initial_pc
+                                      internal_params External.ext
+                                      rule_name_t rules schedule.
+  Parameter correctness : @Core_Common.P_correctness CoreParams.core_id CoreParams.initial_pc
+                                                     internal_params External.ext
+                                                     rule_name_t rules schedule.
+  Parameter compliance : @Core_Common.P_compliance CoreParams.core_id CoreParams.initial_pc
+                                                   internal_params External.ext
+                                                   rule_name_t rules schedule.
 
 End EmptyCore.
